disk-betree/BlockCacheSystem.dfy
@@ -1,0 +1,468 @@
+include "Disk.dfy"
+include "BlockCache.dfy"
+include "../lib/Maps.dfy"
+
+module BlockCacheSystem {
+  import opened Maps
+
+  import M = BlockCache
+  import D = Disk
+
+  type LBA = D.LBA
+  type Sector<T> = D.Sector<T>
+  type DiskOp<T> = D.DiskOp<T>
+
+  datatype Constants = Constants(machine: M.Constants, disk: D.Constants)
+  // TODO TTY
+  // TODO disk message queue for async disk operations
+  datatype Variables<T> = Variables(
+    machine: M.Variables<T>,
+    disk: D.Variables<T>)
+
+  predicate Init(k: Constants, s: Variables)
+  {
+    && M.Init(k.machine, s.machine)
+    && D.Init(k.disk, s.disk)
+  }
+
+  datatype Step<T> =
+    | MachineStep(dop: DiskOp<T>)
+    | CrashStep
+
+  predicate Machine(k: Constants, s: Variables, s': Variables, dop: DiskOp)
+  {
+    && M.Next(k.machine, s.machine, s'.machine, dop)
+    && D.Next(k.disk, s.disk, s'.disk, dop)
+  }
+
+  predicate Crash(k: Constants, s: Variables, s': Variables)
+  {
+    && M.Init(k.machine, s'.machine)
+    && s'.disk == s.disk
+  }
+
+  predicate NextStep(k: Constants, s: Variables, s': Variables, step: Step)
+  {
+    match step {
+      case MachineStep(dop) => Machine(k, s, s', dop)
+      case CrashStep => Crash(k, s, s')
+    }
+  }
+
+  predicate Next<T(!new)>(k: Constants, s: Variables, s': Variables) {
+    exists step :: NextStep(k, s, s', step)
+  }
+
+  // Invariant
+
+  type Superblock = M.Superblock
+  type Reference = M.Reference
+  type Node<T> = M.Node<T>
+
+  predicate WFDisk(k: Constants, blocks: map<LBA, Sector>)
+  {
+    && var superblockLBA := M.SuperblockLBA(k.machine);
+    && superblockLBA in blocks
+    && blocks[superblockLBA].SectorSuperblock?
+    && var superblock := blocks[superblockLBA].superblock;
+    && superblock.refcounts.Keys == superblock.lbas.Keys
+  }
+
+  predicate WFSuperblockWrtDisk(k: Constants, superblock: Superblock, blocks: map<LBA, Sector>)
+  {
+    && (forall ref | ref in superblock.lbas ::
+        && superblock.lbas[ref] in blocks
+        && blocks[superblock.lbas[ref]].SectorBlock?)
+  }
+
+  function DiskSuperblock(k: Constants, blocks: map<LBA, Sector>) : Superblock
+  requires WFDisk(k, blocks)
+  {
+    blocks[M.SuperblockLBA(k.machine)].superblock
+  }
+
+  function RefMapOfDisk(
+      k: Constants,
+      superblock: Superblock,
+      blocks: map<LBA, Sector>) : map<Reference, Node>
+  requires WFDisk(k, blocks)
+  requires WFSuperblockWrtDisk(k, superblock, blocks)
+  {
+    map ref | ref in superblock.lbas :: blocks[superblock.lbas[ref]].block
+  }
+
+  function Graph(superblock: set<Reference>, block: map<Reference, Node>) : map<Reference, Node>
+  requires superblock <= block.Keys
+  {
+    map ref | ref in superblock :: block[ref]
+  }
+
+  function PersistentGraph(k: Constants, s: Variables) : map<Reference, Node>
+  requires WFDisk(k, s.disk.blocks)
+  requires WFSuperblockWrtDisk(k, DiskSuperblock(k, s.disk.blocks), s.disk.blocks)
+  {
+    Graph(
+      DiskSuperblock(k, s.disk.blocks).refcounts.Keys,
+      RefMapOfDisk(k, DiskSuperblock(k, s.disk.blocks), s.disk.blocks))
+  }
+
+  function CacheMap(cache: map<Reference, M.CacheLine>) : map<Reference, Node>
+  {
+    map ref | ref in cache :: cache[ref].block
+  }
+
+  function EphemeralGraph(k: Constants, s: Variables) : map<Reference, Node>
+  requires M.Inv(k.machine, s.machine)
+  requires s.machine.Ready?
+  requires WFDisk(k, s.disk.blocks)
+  requires WFSuperblockWrtDisk(k, s.machine.ephemeralSuperblock, s.disk.blocks)
+  {
+    /*assert s.machine.ephemeralSuperblock.refcounts.Keys
+        <= s.machine.ephemeralSuperblock.lbas.Keys + s.machine.cache.Keys
+        == MapUnionPreferB(RefMapOfDisk(k, s.machine.ephemeralSuperblock, s.disk.blocks), CacheMap(s.machine.cache)).Keys;*/
+    Graph(
+      s.machine.ephemeralSuperblock.refcounts.Keys,
+      MapUnionPreferB(RefMapOfDisk(k, s.machine.ephemeralSuperblock, s.disk.blocks), CacheMap(s.machine.cache))
+    )
+  }
+
+  predicate CleanCacheEntriesAreCorrect(k: Constants, s: Variables)
+  requires s.machine.Ready?
+  {
+    forall ref | ref in s.machine.cache ::
+      ref in s.machine.ephemeralSuperblock.lbas ==>
+      MapsTo(
+          s.disk.blocks,
+          s.machine.ephemeralSuperblock.lbas[ref],
+          M.SectorBlock(s.machine.cache[ref].block))
+  }
+
+  function Predecessors(graph: map<Reference, Node>, ref: Reference) : set<Reference>
+  {
+    set r | r in graph && ref in M.Successors(graph[r])
+  }
+
+  predicate RefcountsAgree(refcounts: map<Reference, int>, graph: map<Reference, Node>)
+  {
+    forall ref | ref in refcounts :: refcounts[ref] == |Predecessors(graph, ref)|
+  }
+
+  predicate NoDanglingPointers(graph: map<Reference, Node>)
+  {
+    forall r1, r2 {:trigger r2 in M.Successors(graph[r1])}
+      | r1 in graph && r2 in M.Successors(graph[r1])
+      :: r2 in graph
+  }
+
+  predicate Inv(k: Constants, s: Variables) {
+    && M.Inv(k.machine, s.machine)
+    && WFDisk(k, s.disk.blocks)
+    && WFSuperblockWrtDisk(k, DiskSuperblock(k, s.disk.blocks), s.disk.blocks)
+    && RefcountsAgree(DiskSuperblock(k, s.disk.blocks).refcounts, PersistentGraph(k, s))
+    && NoDanglingPointers(PersistentGraph(k, s))
+    && (s.machine.Ready? ==>
+      && s.machine.persistentSuperblock == DiskSuperblock(k, s.disk.blocks)
+      && WFSuperblockWrtDisk(k, s.machine.ephemeralSuperblock, s.disk.blocks)
+      && RefcountsAgree(s.machine.ephemeralSuperblock.refcounts, EphemeralGraph(k, s))
+      && NoDanglingPointers(EphemeralGraph(k, s))
+      && CleanCacheEntriesAreCorrect(k, s)
+    )
+  }
+
+  lemma WriteBackStepPreservesInvariant(k: Constants, s: Variables, s': Variables, dop: DiskOp, ref: Reference)
+    requires Inv(k, s)
+    requires M.WriteBack(k.machine, s.machine, s'.machine, dop, ref)
+    requires D.Write(k.disk, s.disk, s'.disk, dop);
+    ensures Inv(k, s')
+  {
+    assert PersistentGraph(k, s) == PersistentGraph(k, s');
+    assert EphemeralGraph(k, s) == EphemeralGraph(k, s');
+  }
+
+  lemma WriteBackSuperblockStepPreservesInvariant(k: Constants, s: Variables, s': Variables, dop: DiskOp)
+    requires Inv(k, s)
+    requires M.WriteBackSuperblock(k.machine, s.machine, s'.machine, dop)
+    requires D.Write(k.disk, s.disk, s'.disk, dop);
+    ensures Inv(k, s')
+  {
+    //assert M.Inv(k.machine, s'.machine);
+    //assert WFDisk(k, s'.disk.blocks);
+    //assert WFSuperblockWrtDisk(k, DiskSuperblock(k, s'.disk.blocks), s'.disk.blocks);
+
+    assert DiskSuperblock(k, s'.disk.blocks) == s.machine.ephemeralSuperblock;
+
+    /*
+    forall ref | ref in CacheMap(s.machine.cache)
+    ensures MapsTo(
+          RefMapOfDisk(k, s.machine.ephemeralSuperblock, s.disk.blocks),
+          ref, CacheMap(s.machine.cache)[ref])
+    {
+    }
+    */
+
+    assert RefMapOfDisk(k, DiskSuperblock(k, s'.disk.blocks), s'.disk.blocks)
+        == RefMapOfDisk(k, s.machine.ephemeralSuperblock, s.disk.blocks)
+        == MapUnionPreferB(RefMapOfDisk(k, s.machine.ephemeralSuperblock, s.disk.blocks), CacheMap(s.machine.cache));
+    assert PersistentGraph(k, s') == EphemeralGraph(k, s);
+
+    //assert RefcountsAgree(DiskSuperblock(k, s'.disk.blocks).refcounts, PersistentGraph(k, s'));
+
+    //assert s'.machine.persistentSuperblock == DiskSuperblock(k, s'.disk.blocks);
+    //assert WFSuperblockWrtDisk(k, s'.machine.ephemeralSuperblock, s'.disk.blocks);
+    //assert RefcountsAgree(s'.machine.ephemeralSuperblock.refcounts, EphemeralGraph(k, s'));
+  }
+
+  lemma RefcountConservation(k: Constants, s: Variables, s': Variables, graph: map<Reference, Node>, graph': map<Reference, Node>, ref: Reference, r: Reference)
+  requires Inv(k, s);
+  requires M.Inv(k.machine, s'.machine)
+  requires s'.machine.Ready?
+  requires s'.disk == s.disk
+  requires WFDisk(k, s'.disk.blocks)
+  requires WFSuperblockWrtDisk(k, s'.machine.ephemeralSuperblock, s'.disk.blocks)
+  requires s.machine.Ready?
+  requires s'.machine.Ready?
+  requires graph == EphemeralGraph(k, s)
+  requires graph' == EphemeralGraph(k, s')
+  requires ref in s.machine.ephemeralSuperblock.lbas ==> ref in s.machine.cache
+  requires ref in s'.machine.ephemeralSuperblock.lbas ==> ref in s'.machine.cache
+  requires MapRemove(s.machine.cache, {ref}) == MapRemove(s'.machine.cache, {ref})
+  requires MapRemove(s.machine.ephemeralSuperblock.lbas, {ref}) == MapRemove(s'.machine.ephemeralSuperblock.lbas, {ref})
+
+  ensures |Predecessors(graph, r)| - (if ref in s.machine.cache && r in M.Successors(s.machine.cache[ref].block) then 1 else 0)
+       == |Predecessors(graph', r)| - (if ref in s'.machine.cache && r in M.Successors(s'.machine.cache[ref].block) then 1 else 0)
+  {
+    assert |Predecessors(graph, r)| - (if ref in s.machine.cache && r in M.Successors(s.machine.cache[ref].block) then 1 else 0) == |Predecessors(graph, r) - {ref}|;
+    assert |Predecessors(graph', r)| - (if ref in s'.machine.cache && r in M.Successors(s'.machine.cache[ref].block) then 1 else 0) == |Predecessors(graph', r) - {ref}|;
+
+    forall r1 | r1 in Predecessors(graph, r) - {ref}
+    ensures r1 in Predecessors(graph', r) - {ref}
+    {
+      assert r1 != ref;
+      if (r1 in s'.machine.ephemeralSuperblock.lbas) {
+        assert r1 in MapRemove(s'.machine.ephemeralSuperblock.lbas, {ref});
+        assert r1 in MapRemove(s.machine.ephemeralSuperblock.lbas, {ref});
+        assert r1 in s.machine.ephemeralSuperblock.lbas;
+        assert s.machine.ephemeralSuperblock.lbas[r1] == 
+               s'.machine.ephemeralSuperblock.lbas[r1];
+        assert RefMapOfDisk(k, s.machine.ephemeralSuperblock, s.disk.blocks)[r1]
+            == RefMapOfDisk(k, s'.machine.ephemeralSuperblock, s'.disk.blocks)[r1];
+      }
+      if (r1 in s.machine.ephemeralSuperblock.lbas) {
+        assert r1 in MapRemove(s.machine.ephemeralSuperblock.lbas, {ref});
+        assert r1 in MapRemove(s'.machine.ephemeralSuperblock.lbas, {ref});
+        assert r1 in s'.machine.ephemeralSuperblock.lbas;
+        assert s'.machine.ephemeralSuperblock.lbas[r1] == 
+               s.machine.ephemeralSuperblock.lbas[r1];
+        assert RefMapOfDisk(k, s.machine.ephemeralSuperblock, s.disk.blocks)[r1]
+            == RefMapOfDisk(k, s'.machine.ephemeralSuperblock, s'.disk.blocks)[r1];
+      }
+
+      if (r1 in s.machine.cache) {
+        assert s.machine.cache.Keys - {ref} == s'.machine.cache.Keys - {ref};
+        assert r1 in (s.machine.cache.Keys - {ref});
+        assert r1 in (s'.machine.cache.Keys - {ref});
+        assert r1 in s'.machine.cache;
+        assert graph[r1] == s.machine.cache[r1].block
+            == s'.machine.cache[r1].block
+            == graph'[r1];
+        assert MapsTo(graph', r1, graph[r1]);
+      } else {
+        assert MapsTo(graph', r1, graph[r1]);
+      }
+      assert r1 in Predecessors(graph', r) - {ref};
+    }
+
+    forall r1 | r1 in Predecessors(graph', r) - {ref}
+    ensures r1 in Predecessors(graph, r) - {ref}
+    {
+      assert r1 != ref;
+      if (r1 in s'.machine.cache) {
+        assert MapsTo(graph, r1, graph[r1]);
+      } else {
+        assert MapsTo(graph, r1, graph[r1]);
+      }
+      assert r1 in Predecessors(graph, r) - {ref};
+    }
+
+    assert Predecessors(graph, r) - {ref} == Predecessors(graph', r) - {ref};
+  }
+
+  lemma DirtyStepPreservesInvariant(k: Constants, s: Variables, s': Variables, dop: DiskOp, ref: Reference, block: Node)
+    requires Inv(k, s)
+    requires M.Dirty(k.machine, s.machine, s'.machine, dop, ref, block)
+    requires D.Stutter(k.disk, s.disk, s'.disk, dop);
+    ensures Inv(k, s')
+  {
+    var refcounts := s.machine.ephemeralSuperblock.refcounts;
+    var refcounts' := s'.machine.ephemeralSuperblock.refcounts;
+    var graph := EphemeralGraph(k, s);
+    var graph' := EphemeralGraph(k, s');
+    var cache := s.machine.cache;
+    var cache' := s'.machine.cache;
+
+    forall r | r in refcounts'
+    ensures refcounts'[r] == |Predecessors(graph', r)|
+    {
+      RefcountConservation(k, s, s', graph, graph', ref, r);
+
+      /*
+      assert refcounts'[r]
+          == refcounts[r] +
+            (if ref in cache' && r in M.Successors(cache'[ref].block) then 1 else 0) -
+            (if ref in cache && r in M.Successors(cache[ref].block) then 1 else 0)
+          == |Predecessors(graph, r)| +
+            (if ref in cache' && r in M.Successors(cache'[ref].block) then 1 else 0) -
+            (if ref in cache && r in M.Successors(cache[ref].block) then 1 else 0)
+          == |Predecessors(graph', r)|;
+      */
+    }
+  }
+
+  lemma AllocStepPreservesInvariant(k: Constants, s: Variables, s': Variables, dop: DiskOp, ref: Reference, block: Node)
+    requires Inv(k, s)
+    requires M.Alloc(k.machine, s.machine, s'.machine, dop, ref, block)
+    requires D.Stutter(k.disk, s.disk, s'.disk, dop);
+    ensures Inv(k, s')
+  {
+    var refcounts := s.machine.ephemeralSuperblock.refcounts;
+    var refcounts' := s'.machine.ephemeralSuperblock.refcounts;
+    var graph := EphemeralGraph(k, s);
+    var graph' := EphemeralGraph(k, s');
+    var cache := s.machine.cache;
+    var cache' := s'.machine.cache;
+
+    forall r | r in refcounts'
+    ensures refcounts'[r] == |Predecessors(graph', r)|
+    {
+      if (r == ref) {
+        //assert ref !in M.Successors(block);
+        //assert ref !in s.machine.cache;
+        //assert ref !in M.Successors(s'.machine.cache[ref].block);
+
+        RefcountConservation(k, s, s', graph, graph', ref, r);
+        /*if (|Predecessors(graph, r)| != 0) {
+          var x :| x in Predecessors(graph, r);
+          assert r in M.Successors(graph[x]);
+          assert r in graph;
+          assert false;
+        }*/
+        assert |Predecessors(graph, r)| == 0;
+
+        assert |Predecessors(graph', r)| == 0;
+        assert refcounts'[r] == 0;
+      } else {
+        RefcountConservation(k, s, s', graph, graph', ref, r);
+      }
+    }
+
+    /*forall r1, r2 | r1 in graph && r2 in M.Successors(graph[r1])
+    ensures r2 in graph'
+    {
+      /*
+      if (r_node in graph) {
+        assert node in graph.Values;
+        assume false;
+        assert r in graph;
+        assert r in graph';
+      } else {
+        assume false;
+        assert node == block;
+        assert r in graph;
+        assert r in graph';
+      }
+      */
+    }*/
+  }
+
+  lemma UnallocStepPreservesInvariant(k: Constants, s: Variables, s': Variables, dop: DiskOp, ref: Reference)
+    requires Inv(k, s)
+    requires M.Unalloc(k.machine, s.machine, s'.machine, dop, ref)
+    requires D.Stutter(k.disk, s.disk, s'.disk, dop);
+    ensures Inv(k, s')
+  {
+    var refcounts := s.machine.ephemeralSuperblock.refcounts;
+    var refcounts' := s'.machine.ephemeralSuperblock.refcounts;
+    var graph := EphemeralGraph(k, s);
+    var graph' := EphemeralGraph(k, s');
+    var cache := s.machine.cache;
+    var cache' := s'.machine.cache;
+
+    forall r | r in refcounts'
+    ensures refcounts'[r] == |Predecessors(graph', r)|
+    {
+      assert r != ref;
+      RefcountConservation(k, s, s', graph, graph', ref, r);
+    }
+  }
+
+  lemma PageInStepPreservesInvariant(k: Constants, s: Variables, s': Variables, dop: DiskOp, ref: Reference)
+    requires Inv(k, s)
+    requires M.PageIn(k.machine, s.machine, s'.machine, dop, ref)
+    requires D.Read(k.disk, s.disk, s'.disk, dop);
+    ensures Inv(k, s')
+  {
+  }
+
+  lemma PageInSuperblockStepPreservesInvariant(k: Constants, s: Variables, s': Variables, dop: DiskOp)
+    requires Inv(k, s)
+    requires M.PageInSuperblock(k.machine, s.machine, s'.machine, dop)
+    requires D.Read(k.disk, s.disk, s'.disk, dop);
+    ensures Inv(k, s')
+  {
+  }
+
+  lemma EvictStepPreservesInvariant(k: Constants, s: Variables, s': Variables, dop: DiskOp, ref: Reference)
+    requires Inv(k, s)
+    requires M.Evict(k.machine, s.machine, s'.machine, dop, ref)
+    requires D.Stutter(k.disk, s.disk, s'.disk, dop);
+    ensures Inv(k, s')
+  {
+    assert EphemeralGraph(k, s) == EphemeralGraph(k, s');
+  }
+
+  lemma MachineStepPreservesInvariant(k: Constants, s: Variables, s': Variables, dop: DiskOp)
+    requires Inv(k, s)
+    requires Machine(k, s, s', dop)
+    ensures Inv(k, s')
+  {
+    var step :| M.NextStep(k.machine, s.machine, s'.machine, dop, step);
+    match step {
+      case WriteBackStep(ref) => WriteBackStepPreservesInvariant(k, s, s', dop, ref);
+      case WriteBackSuperblockStep => WriteBackSuperblockStepPreservesInvariant(k, s, s', dop);
+      case DirtyStep(ref, block) => DirtyStepPreservesInvariant(k, s, s', dop, ref, block);
+      case AllocStep(ref, block) => AllocStepPreservesInvariant(k, s, s', dop, ref, block);
+      case UnallocStep(ref) => UnallocStepPreservesInvariant(k, s, s', dop, ref);
+      case PageInStep(ref) => PageInStepPreservesInvariant(k, s, s', dop, ref);
+      case PageInSuperblockStep => PageInSuperblockStepPreservesInvariant(k, s, s', dop);
+      case EvictStep(ref) => EvictStepPreservesInvariant(k, s, s', dop, ref);
+    }
+  }
+
+  lemma CrashStepPreservesInvariant(k: Constants, s: Variables, s': Variables)
+    requires Inv(k, s)
+    requires Crash(k, s, s')
+    ensures Inv(k, s')
+  {
+  }
+
+  lemma NextStepPreservesInvariant(k: Constants, s: Variables, s': Variables, step: Step)
+    requires Inv(k, s)
+    requires NextStep(k, s, s', step)
+    ensures Inv(k, s')
+  {
+    match step {
+      case MachineStep(dop: DiskOp) => MachineStepPreservesInvariant(k, s, s', dop);
+      case CrashStep => CrashStepPreservesInvariant(k, s, s');
+    }
+  }
+
+  lemma NextPreservesInv(k: Constants, s: Variables, s': Variables)
+    requires Inv(k, s)
+    requires Next(k, s, s')
+    ensures Inv(k, s')
+  {
+    var step :| NextStep(k, s, s', step);
+    NextStepPreservesInvariant(k, s, s', step);
+  }
+
+}
