disk-betree/Disk.dfy
@@ -1,0 +1,52 @@
+include "BlockCache.dfy"
+include "../lib/Maps.dfy"
+
+module Disk {
+  import BC = BlockCache
+  import opened Maps
+
+  type LBA = BC.LBA
+  type Sector<T> = BC.Sector<T>
+  type DiskOp<T> = BC.DiskOp<T>
+
+  datatype Constants = Constants()
+  datatype Variables<T> = Variables(blocks: map<LBA, Sector<T>>)
+
+  predicate Init(k: Constants, s: Variables)
+  {
+    true // TODO
+  }
+
+  datatype Step =
+    | WriteStep
+    | ReadStep
+    | StutterStep
+
+  predicate Write(k: Constants, s: Variables, s': Variables, dop: DiskOp) {
+    && dop.Write?
+    && s'.blocks == s.blocks[dop.lba := dop.sector]
+  }
+
+  predicate Read(k: Constants, s: Variables, s': Variables, dop: DiskOp) {
+    && dop.Write?
+    && s' == s
+    && MapsTo(s.blocks, dop.lba, dop.sector)
+  }
+
+  predicate Stutter(k: Constants, s: Variables, s': Variables, dop: DiskOp) {
+    && dop.NoDiskOp?
+    && s' == s
+  }
+
+  predicate NextStep(k: Constants, s: Variables, s': Variables, dop: DiskOp, step: Step) {
+    match step {
+      case WriteStep => Write(k, s, s', dop)
+      case ReadStep => Read(k, s, s', dop)
+      case StutterStep => Stutter(k, s, s', dop)
+    }
+  }
+
+  predicate Next(k: Constants, s: Variables, s': Variables, dop: DiskOp) {
+    exists step :: NextStep(k, s, s', dop, step)
+  }
+}
